Working on new version of alpha conversion
Function only changes specific vars according to given map
Different (not stronger or weaker) from previous version
Proved alpha equivalence
In process of proving bound vars, did let and match case

proofs/core/Alpha.v
@@ -6207,19 +6207,21 @@ End Shape.
   and show it has all the nice properties we want*)
 Section ConvertFn.
 
-Definition a_convert_t (t: term) :=
-  alpha_t_aux t (gen_strs (length (tm_bnd t)) (tm_bnd t ++ tm_fv t)).
-Definition a_convert_f (f: formula) :=
-  alpha_f_aux f (gen_strs (length (fmla_bnd f)) (fmla_bnd f ++ fmla_fv f)).
+(*Alpha convert the term t and give new bound variables not in l*)
+Definition a_convert_t (t: term) (l: list vsymbol) :=
+  alpha_t_aux t (gen_strs (length (tm_bnd t)) (l ++ tm_bnd t ++ tm_fv t)).
+
+Definition a_convert_f (f: formula) (l: list vsymbol) :=
+  alpha_f_aux f (gen_strs (length (fmla_bnd f)) (l ++ fmla_bnd f ++ fmla_fv f)).
 
 (*Correctness*)
-Theorem a_convert_t_wf t :
-  term_wf (a_convert_t t).
+Theorem a_convert_t_wf t l :
+  term_wf (a_convert_t t l).
 Proof.
   unfold term_wf.
-  pose proof (gen_strs_nodup (length (tm_bnd t)) (tm_bnd t ++ tm_fv t)) as Hnodup.
-  pose proof (gen_strs_length (length (tm_bnd t)) (tm_bnd t ++ tm_fv t)) as Hlen.
-  pose proof (gen_strs_notin (length (tm_bnd t)) (tm_bnd t ++ tm_fv t)) as Hnotin.
+  pose proof (gen_strs_nodup (length (tm_bnd t)) (l ++ tm_bnd t ++ tm_fv t)) as Hnodup.
+  pose proof (gen_strs_length (length (tm_bnd t)) (l ++ tm_bnd t ++ tm_fv t)) as Hlen.
+  pose proof (gen_strs_notin (length (tm_bnd t)) (l ++ tm_bnd t ++ tm_fv t)) as Hnotin.
   split.
   - apply alpha_t_aux_bnd; auto.
   - intros x [Hinx1 Hinx2].
@@ -6229,8 +6231,8 @@ Proof.
     apply Hnotin in Hinx2. apply Hinx2. in_tac.
 Qed.
 
-Theorem a_convert_t_equiv t:
-  a_equiv_t t (a_convert_t t).
+Theorem a_convert_t_equiv t l:
+  a_equiv_t t (a_convert_t t l).
 Proof.
   apply alpha_t_aux_equiv; 
   [apply gen_strs_nodup | apply gen_strs_length | |];
@@ -6238,18 +6240,18 @@ Proof.
 Qed.
 
 (*And the corollaries:*)
-Corollary a_convert_t_ty t ty:
+Corollary a_convert_t_ty t l ty:
   term_has_type gamma t ty ->
-  term_has_type gamma (a_convert_t t) ty.
+  term_has_type gamma (a_convert_t t l) ty.
 Proof.
   apply a_equiv_t_type.
   apply a_convert_t_equiv.
 Qed.
 
-Corollary a_convert_t_rep v t ty 
+Corollary a_convert_t_rep v t l ty 
   (Hty: term_has_type gamma t ty):
   term_rep v t ty Hty = 
-  term_rep v (a_convert_t t) ty (a_convert_t_ty t ty Hty).
+  term_rep v (a_convert_t t l) ty (a_convert_t_ty t l ty Hty).
 Proof.
   apply a_equiv_t_equiv.
   apply a_convert_t_equiv.
@@ -6257,13 +6259,13 @@ Qed.
 
 (*And likewise for formulas*)
 
-Theorem a_convert_f_wf f :
-  fmla_wf (a_convert_f f).
+Theorem a_convert_f_wf f l:
+  fmla_wf (a_convert_f f l).
 Proof.
   unfold fmla_wf.
-  pose proof (gen_strs_nodup (length (fmla_bnd f)) (fmla_bnd f ++ fmla_fv f)) as Hnodup.
-  pose proof (gen_strs_length (length (fmla_bnd f)) (fmla_bnd f ++ fmla_fv f)) as Hlen.
-  pose proof (gen_strs_notin (length (fmla_bnd f)) (fmla_bnd f ++ fmla_fv f)) as Hnotin.
+  pose proof (gen_strs_nodup (length (fmla_bnd f)) (l ++ fmla_bnd f ++ fmla_fv f)) as Hnodup.
+  pose proof (gen_strs_length (length (fmla_bnd f)) (l ++ fmla_bnd f ++ fmla_fv f)) as Hlen.
+  pose proof (gen_strs_notin (length (fmla_bnd f)) (l ++ fmla_bnd f ++ fmla_fv f)) as Hnotin.
   split.
   - apply alpha_f_aux_bnd; auto.
   - intros x [Hinx1 Hinx2].
@@ -6273,8 +6275,8 @@ Proof.
     apply Hnotin in Hinx2. apply Hinx2. in_tac.
 Qed.
 
-Theorem a_convert_f_equiv f:
-  a_equiv_f f (a_convert_f f).
+Theorem a_convert_f_equiv f l:
+  a_equiv_f f (a_convert_f f l).
 Proof.
   apply alpha_f_aux_equiv;
   [apply gen_strs_nodup | apply gen_strs_length | |];
@@ -6282,35 +6284,35 @@ Proof.
 Qed.
 
 (*And the corollaries:*)
-Corollary a_convert_f_valid f:
+Corollary a_convert_f_valid f l:
   formula_typed gamma f ->
-  formula_typed gamma (a_convert_f f).
+  formula_typed gamma (a_convert_f f l).
 Proof.
   apply a_equiv_f_valid.
   apply a_convert_f_equiv.
 Qed.
 
-Corollary a_convert_f_rep v f 
+Corollary a_convert_f_rep v f l 
   (Hval: formula_typed gamma f):
   formula_rep v f Hval = 
-  formula_rep v (a_convert_f f) (a_convert_f_valid f Hval).
+  formula_rep v (a_convert_f f l) (a_convert_f_valid f l Hval).
 Proof.
   apply a_equiv_f_equiv.
   apply a_convert_f_equiv.
 Qed.
 
-Corollary a_convert_f_valid_ind_form p f:
+Corollary a_convert_f_valid_ind_form p f l:
   valid_ind_form p f ->
-  valid_ind_form p (a_convert_f f).
+  valid_ind_form p (a_convert_f f l).
 Proof.
   intros. eapply shape_ind_form. 2: apply H.
   apply alpha_shape_f with(vars:=nil).
   apply a_convert_f_equiv.
 Qed.
 
-Corollary a_convert_f_pos ps f:
+Corollary a_convert_f_pos ps f l:
   ind_positive ps f ->
-  ind_positive ps (a_convert_f f).
+  ind_positive ps (a_convert_f f l).
 Proof.
   intros. eapply shape_ind_positive. 2: apply H.
   apply alpha_shape_f with (vars:=nil).
@@ -6318,5 +6320,578 @@ Proof.
 Qed.
 
 End ConvertFn.
+
+(*1 attempt - let's see if it works*)
+
+(*Instead of replacing all variables, replace bound vars
+  according to map - leave others unchanged. This does NOT
+  give wf, but may make things more readable*)
+
+Definition replace_var (l: list (string * string)) (x: vsymbol) : vsymbol :=
+  match (get_assoc_list string_dec l (fst x)) with
+  | Some y => (y, snd x)
+  | None => x
+  end.
+
+Lemma replace_var_ty l x:
+  snd (replace_var l x) = snd x.
+Proof.
+  unfold replace_var.
+  destruct (get_assoc_list string_dec l (fst x)); auto.
+Qed.
+
+Definition a_convert_map_p (l: list (string * string)) (p: pattern) :
+  pattern :=
+  map_pat (replace_var l) p.
+
+
+(*Fixpoint a_convert_map_p (l: list (string * string)) 
+  (p: pattern) : pattern :=
+  match p with
+  | Pvar v =>
+    Pvar (replace_var l v)
+  | Pconstr f tys ps =>
+    Pconstr f tys (map (a_convert_map_p l) ps)
+  | Pwild => Pwild
+  | Por p1 p2 => Por (a_convert_map_p l p1) (a_convert_map_p l p2)
+  | Pbind p1 v => Pbind (a_convert_map_p l p1) (replace_var l v)
+  end.
+
+(*TODO: is this better definitoin?*)
+Lemma a_convert_map_p_eq l p:
+  a_convert_map_p l p =
+  map_pat (replace_var l) p.
+Proof.
+  induction p; simpl; auto.
+  - f_equal. induction ps; simpl; auto;
+    inversion H; subst; auto.
+    rewrite H2, IHps; auto.
+  - rewrite IHp1, IHp2; auto.
+  - rewrite IHp; auto.
+Qed.*)
+
+
+
+(*Lemma big_union_map {A B C: Type} (eq_dec: forall (x y: A), {x = y} + {x <> y})
+  (f: B -> list A) (l: list B)
+  (g: B -> B) (h: A -> A)
+  (Hcompat: Forall (fun x => )):
+  big_union eq_dec f (map g l) =
+  map g (big_union eq_dec f l).*)
+
+Lemma replace_var_inj l x y
+  (Hn: NoDup (map snd l)):
+  ~ In (fst x) (map snd l) ->
+  ~ In (fst y) (map snd l) ->
+  replace_var l x = replace_var l y ->
+  x = y.
+Proof.
+  intros. unfold replace_var in H1.
+  destruct x as [x1 x2]; destruct y as [y1 y2]; simpl in *; subst.
+  destruct (get_assoc_list string_dec l x1) eqn : Hx;
+  destruct (get_assoc_list string_dec l y1) eqn : Hy; auto;
+  inversion H1; subst.
+  - apply get_assoc_list_some in Hx, Hy.
+    pose proof (NoDup_map_in Hn Hx Hy eq_refl).
+    inversion H2; subst; auto.
+  - apply get_assoc_list_some in Hx.
+    exfalso. 
+    apply H0. rewrite in_map_iff. exists (x1, y1); auto. 
+  - apply get_assoc_list_some in Hy.
+    exfalso.
+    apply H. rewrite in_map_iff. exists (y1, s); auto.
+Qed.
+
+Lemma a_convert_map_p_fv l p
+  (Hn: NoDup (map snd l))
+  (Hfv: forall x, In x (pat_fv p) -> ~ In (fst x) (map snd l)):
+  pat_fv (a_convert_map_p l p) =
+  map (replace_var l) (pat_fv p).
+Proof.
+  unfold a_convert_map_p.
+  apply map_pat_free_vars.
+  intros x y Hx Hy.
+  apply Hfv in Hx, Hy.
+  apply replace_var_inj; auto.
+Qed.
+
+
+
+
+
+(*
+
+  induction p; simpl; auto.
+  - simpl in Hfv. induction ps; simpl in *; auto.
+    inversion H; subst.
+    erewrite map_union. f_equal; auto.
+    + apply H2. intros; apply Hfv; simpl_set; auto.
+    + apply IHps; auto; intros; apply Hfv; simpl_set; auto.
+    + intros x y. rewrite !in_app_iff, <- !(union_elts vsymbol_eq_dec).
+      intros Hx Hy.
+      apply replace_var_inj; auto.
+  - simpl in Hfv. rewrite (map_union _ vsymbol_eq_dec); auto.
+    + rewrite IHp1, IHp2; auto; intros; apply Hfv; simpl_set; auto.
+    + intros x y. rewrite !in_app_iff, <- !(union_elts vsymbol_eq_dec).
+      intros Hx Hy. apply Hfv in Hx, Hy.
+      apply replace_var_inj; auto.
+  - simpl in Hfv.
+    rewrite (map_union _ vsymbol_eq_dec).
+    + rewrite IHp; auto; intros; apply Hfv; simpl_set; auto.
+    + intros x y. rewrite !in_app_iff, <- !(union_elts vsymbol_eq_dec);
+      intros Hx Hy. apply Hfv in Hx, Hy. apply replace_var_inj; auto.
+Qed.*)
+
+(*This proof is easy because we just map*)
+Lemma a_convert_alpha_p (l: list (string * string))
+  (p: pattern)
+  (Hn: NoDup (map snd l))
+  (Hfv: forall x, In x (pat_fv p) -> ~ In (fst x) (map snd l)):
+  alpha_equiv_p (combine (pat_fv p) 
+    (pat_fv (a_convert_map_p l p)))
+    p (a_convert_map_p l p).
+Proof.
+  apply map_pat_alpha_equiv.
+  - intros; rewrite replace_var_ty; auto.
+  - intros x Hinx.
+    rewrite a_convert_map_p_fv; auto.
+    induction (pat_fv p); simpl in *; auto.
+    vsym_eq x a; simpl.
+    + rewrite eq_dec_refl; auto.
+    + destruct Hinx; subst; try contradiction.
+      vsym_eq (replace_var l x) (replace_var l a).
+      exfalso.
+      apply replace_var_inj in e; auto.
+Qed.
+
+Fixpoint a_convert_map_t (l: list (string * string))
+  (bnd: list vsymbol) (t: term) : term :=
+  match t with
+  | Tvar v =>
+    Tvar (if in_bool vsymbol_eq_dec v bnd then 
+    replace_var l v else v)
+  | Tfun fs tys tms => Tfun fs tys (map (a_convert_map_t l bnd) tms)
+  | Tlet t1 v t2 =>
+    Tlet (a_convert_map_t l bnd t1) (replace_var l v) 
+      (a_convert_map_t l (v :: bnd) t2)
+  | Tif f1 t1 t2 =>
+    Tif (a_convert_map_f l bnd f1) (a_convert_map_t l bnd t1) (a_convert_map_t l bnd t2)
+  | Tmatch tm ty ps =>
+    Tmatch (a_convert_map_t l bnd tm) ty
+      (map (fun x => (a_convert_map_p l (fst x), 
+        (a_convert_map_t l (pat_fv (fst x) ++ bnd) (snd x)))) ps)
+  | Teps f v => Teps (a_convert_map_f l (v :: bnd) f) (replace_var l v)
+  | _ => t
+  end
+with a_convert_map_f (l: list (string * string)) 
+  (bnd: list vsymbol) (f: formula) : formula :=
+  match f with
+  | Fpred p tys tms => Fpred p tys (map (a_convert_map_t l bnd) tms)
+  | Fquant q v f => Fquant q (replace_var l v) (a_convert_map_f l (v :: bnd) f)
+  | Feq ty t1 t2 => Feq ty (a_convert_map_t l bnd t1) (a_convert_map_t l bnd t2)
+  | Fbinop b f1 f2 => Fbinop b (a_convert_map_f l bnd f1) (a_convert_map_f l bnd f2)
+  | Fnot f => Fnot (a_convert_map_f l bnd f)
+  | Flet t v f => Flet (a_convert_map_t l bnd t) (replace_var l v)
+    (a_convert_map_f l (v :: bnd) f)
+  | Fif f1 f2 f3 => Fif (a_convert_map_f l bnd f1) (a_convert_map_f l  bnd f2)
+    (a_convert_map_f l bnd f3)
+  | Fmatch tm ty ps =>
+    Fmatch (a_convert_map_t l bnd tm) ty
+    (map (fun x => (a_convert_map_p l (fst x), 
+      (a_convert_map_f l (pat_fv (fst x) ++ bnd) (snd x)))) ps)
+  | _ => f
+  end.
+
+Definition mk_alpha_list (l: list (string * string)) (bnd: list vsymbol) :=
+  map (fun v => (v, replace_var l v)) bnd.
+
+(*Actually, we need l to encompass all variables in bnd
+  This is OK, we can always add the identity for vars we don't want
+  to change. Otherwise, we can have the following bad situation:
+  forall x, exists y, y + x = 2
+  say: x -> y, then we have forall y, exists y, y + y = 2
+  *)
+Lemma mk_alpha_list_in  (l: list (string * string)) (bnd: list vsymbol)
+  (Hn: NoDup (map snd l))
+  (Hall: forall x, In x bnd -> In (fst x) (map fst l)) v:
+  In v bnd ->
+  eq_var (mk_alpha_list l bnd) v (replace_var l v).
+Proof.
+  intros.
+  induction bnd; simpl. destruct H.
+  vsym_eq v a; simpl; try rewrite eq_dec_refl; auto.
+  destruct H; subst; auto. simpl in Hall.
+  vsym_eq (replace_var l v) (replace_var l a); simpl.
+  unfold replace_var in e.
+  destruct v as [v1 v2]; destruct a as [a1 a2]; subst; simpl in *.
+  exfalso.
+  destruct (get_assoc_list string_dec l v1) eqn : Hv.
+  2: {
+    rewrite get_assoc_list_none in Hv. apply Hv.
+    apply (Hall (v1, v2)); auto.
+  }
+  destruct (get_assoc_list string_dec l a1) eqn : Ha.
+  2: {
+    rewrite get_assoc_list_none in Ha. apply Ha.
+    apply (Hall (a1, a2)); auto.
+  }
+  inversion e; subst.
+  apply get_assoc_list_some in Hv, Ha.
+  f_equal.
+  pose proof (NoDup_map_in Hn Hv Ha eq_refl).
+  inversion H0; subst; auto.
+Qed.
+
+Lemma mk_alpha_list_in'  (l: list (string * string)) (bnd: list vsymbol)
+  (Hn: NoDup (map snd l))
+  (Hall: forall x, In x bnd -> ~ In (fst x) (map snd l))
+  (*(Hall: forall x, In x bnd -> In (fst x) (map fst l))*) v:
+  In v bnd ->
+  (*~ In (fst v) (map snd l) ->*)
+  eq_var (mk_alpha_list l bnd) v (replace_var l v).
+Proof.
+  intros.
+  induction bnd; simpl. destruct H.
+  vsym_eq v a; simpl; try rewrite eq_dec_refl; auto.
+  simpl in Hall.
+  destruct H; subst; auto.
+  vsym_eq (replace_var l v) (replace_var l a); simpl.
+  apply replace_var_inj in e; auto.
+Qed.
+
+Lemma mk_alpha_list_notin (l: list (string * string)) (bnd: list vsymbol) 
+v:
+~ In (fst v) (map snd l) ->
+~ In v bnd ->
+eq_var (mk_alpha_list l bnd) v v.
+Proof.
+  intros. induction bnd; simpl. vsym_eq v v.
+  simpl in H0. not_or Hv.
+  vsym_eq v a; simpl.
+  destruct (vsymbol_eq_dec v (replace_var l a)); simpl; auto.
+  unfold replace_var in e.
+  destruct v as [v1 v2]; destruct a as [a1 a2]; simpl in *.
+  destruct (get_assoc_list string_dec l a1) eqn : Ha.
+  - inversion e; subst.
+    apply get_assoc_list_some in Ha.
+    exfalso. apply H. rewrite in_map_iff. exists (a1, s); auto.
+  - contradiction.
+Qed.
+
+(*Need the free var condition because otherwise, we can 
+  capture free vars: ex:
+  forall x, x + y ... then x -> y
+  becomes forall y, y + y*)
+
+  (*We need the following condition: every pair in l is 
+  either: (v, v) for v bound in t OR
+  (x, y) for x bound in t and y not appearing in t*)
+
+Ltac solve_invars Hfree Hbnd1 Hbnd2 := 
+  let x := fresh  "x" in
+  let Hinx := fresh "Hinx" in
+  intros x Hinx;
+  try (solve[apply (Hfree x); simpl_set; auto;
+  match goal with
+  | H: In x (tm_fv (nth ?i ?l1 ?d)) |- 
+    exists y, In y ?l1 /\ In x (tm_fv y) =>
+    exists (nth i l1 d); auto
+  end
+  ]);
+  try (solve[apply (Hbnd1 x); try rewrite in_concat; 
+    try rewrite !in_app_iff; 
+  try rewrite in_map_iff; auto;
+  match goal with
+  | H: In x (tm_bnd (nth ?i ?l1 ?d)) |- 
+    exists l, In l (map tm_bnd ?l1) /\ In x l =>
+    exists (tm_bnd (nth i l1 d)); split; auto;
+    rewrite in_map_iff;
+    exists (nth i l1 d); auto
+  end
+  ]);
+  try (solve[destruct Hinx; subst; auto]). 
+
+Ltac bnd_case v Hfree :=
+  let x := fresh "x" in
+  let Hinx := fresh "Hinx" in
+  intros x Hinx;
+  vsym_eq x v;
+  apply Hfree; simpl_set; auto.
+
+(*Then we prove alpha equivalence. The proof is easier than above,
+  since this is just a map. Only the match cases are a bit annoying*)
+Lemma a_convert_alpha (l: list (string * string))
+  (Hn: NoDup (map snd l))
+  (t: term) (f: formula) :
+  (forall bnd
+    (Hfree: forall x, In x (tm_fv t) -> ~ In (fst x) (map snd l))
+    (Hbnd1: forall x, In x (tm_bnd t) -> ~ In (fst x) (map snd l))
+    (Hbnd2: forall x, In x bnd -> ~ In (fst x) (map snd l)), 
+    alpha_equiv_t (mk_alpha_list l bnd) t (a_convert_map_t l bnd t)) /\
+  (forall bnd
+    (Hfree: forall x, In x (fmla_fv f) -> ~ In (fst x) (map snd l))
+    (Hbnd1: forall x, In x (fmla_bnd f) -> ~ In (fst x) (map snd l))
+    (Hbnd2: forall x, In x bnd -> ~ In (fst x) (map snd l)),
+    alpha_equiv_f (mk_alpha_list l bnd) f (a_convert_map_f l bnd f)).
+Proof.
+  revert t f; apply term_formula_ind; simpl; intros; auto.
+  - apply eq_dec_refl.
+  - (*Tvar*) destruct (in_bool_spec vsymbol_eq_dec v bnd).
+    + apply mk_alpha_list_in'; auto.
+    + apply mk_alpha_list_notin; auto.
+  - (*Tfun*) rewrite map_length, !eq_dec_refl, Nat.eqb_refl. simpl.
+    rewrite all2_forall with(d1:=tm_d)(d2:=tm_d); [|rewrite map_length; auto].
+    intros i Hi.
+    rewrite Forall_forall in H.
+    rewrite map_nth_inbound with (d2:=tm_d); auto.
+    assert (Hin: In (nth i l1 tm_d) l1) by (apply nth_In; auto).
+    apply H; auto; solve_invars Hfree Hbnd1 Hbnd2.
+  - (*Tlet*) simpl. rewrite replace_var_ty, eq_dec_refl. simpl.
+    rewrite H; auto.
+    2: { bnd_case v Hfree. }
+    2: { solve_invars Hfree Hbnd1 Hbnd2. } 
+    simpl.
+    apply (H0 (v :: bnd)); simpl; [bnd_case v Hfree | |];
+      solve_invars Hfree Hbnd1 Hbnd2.
+  - (*Tif*) rewrite H, H0, H1; auto;  solve_invars Hfree Hbnd1 Hbnd2.
+  - (*Tmatch*) rewrite H; auto; try solve[solve_invars Hfree Hbnd1 Hbnd2].
+    simpl. rewrite map_length, Nat.eqb_refl, eq_dec_refl. simpl.
+    rewrite all2_forall with(d1:=(Pwild, tm_d))(d2:=(Pwild, tm_d)).
+    2: rewrite map_length; auto.
+    intros i Hi.
+    rewrite map_nth_inbound with (d2:=(Pwild, tm_d)); auto. simpl.
+    set (t := (nth i ps (Pwild, tm_d))) in *.
+    (*Results we need*)
+    assert (Hint: In t ps). {
+      apply nth_In; auto.
+    }
+    assert (Hbndi: forall x, In x (pat_fv (fst t)) \/ In x (tm_bnd (snd t)) ->
+    ~ In (fst x) (map snd l)). {
+      intros. apply Hbnd1; rewrite !in_app_iff, in_concat.
+      right. exists (pat_fv (fst t) ++ tm_bnd (snd t)).
+      split; [rewrite in_map_iff |
+      rewrite in_app_iff]; auto.
+      exists t. split; auto.
+    }
+    assert (Hfvi: forall x, In x (tm_fv (snd t)) ->
+      ~ In (fst x) (map snd l)). {
+      intros x Hinx.
+      destruct (in_bool_spec vsymbol_eq_dec x (pat_fv (fst t))); auto.
+      apply Hfree. simpl_set. right.
+      exists t. split; auto. simpl_set; auto.
+    }
+    rewrite a_convert_alpha_p; auto; simpl.
+    rewrite Forall_map in H0.
+    rewrite Forall_forall in H0.
+    unfold add_vals.
+    rewrite a_convert_map_p_fv; auto.
+    replace (combine (pat_fv (fst t))
+    (map (replace_var l) (pat_fv (fst t))) ++
+    mk_alpha_list l bnd) with 
+    (mk_alpha_list l (pat_fv (fst t) ++ bnd)) .
+    2: {
+      unfold mk_alpha_list. rewrite map_app.
+      f_equal.
+      rewrite <- (combine_eq (map _ _)).
+      rewrite !map_map. simpl. f_equal.
+      rewrite map_id; auto.
+    }
+    apply H0; auto.
+    intros x. rewrite in_app_iff; intros [Hx | Hx]; auto.
+  - (*Teps*) rewrite replace_var_ty, eq_dec_refl. simpl.
+    apply (H (v :: bnd)); simpl;[bnd_case v Hfree | |];
+    solve_invars Hfree Hbnd1 Hbnd2.
+  - (*Fpred*)
+    rewrite map_length, !eq_dec_refl, Nat.eqb_refl. simpl.
+    rewrite all2_forall with(d1:=tm_d)(d2:=tm_d); [|rewrite map_length; auto].
+    intros i Hi.
+    rewrite Forall_forall in H.
+    rewrite map_nth_inbound with (d2:=tm_d); auto.
+    assert (Hin: In (nth i tms tm_d) tms) by (apply nth_In; auto).
+    apply H; auto; solve_invars Hfree Hbnd1 Hbnd2.
+  - (*Fquant*) rewrite replace_var_ty, !eq_dec_refl. simpl.
+    apply (H (v :: bnd)); simpl;[bnd_case v Hfree | |];
+    solve_invars Hfree Hbnd1 Hbnd2.
+  - (*Feq*)
+    rewrite eq_dec_refl, H, H0; auto;
+    solve_invars Hfree Hbnd1 Hbdn2.
+  - (*binop*)
+    rewrite eq_dec_refl, H, H0; auto;
+    solve_invars Hfree Hbnd1 Hbdn2.
+  - (*Flet*) rewrite replace_var_ty, eq_dec_refl. simpl.
+    rewrite H; auto; [|bnd_case v Hfree | solve_invars Hfree Hbnd1 Hbnd2].
+    simpl.
+    apply (H0 (v :: bnd)); simpl; [bnd_case v Hfree | |];
+      solve_invars Hfree Hbnd1 Hbnd2.
+  - (*Fif*) rewrite H, H0, H1; auto; solve_invars Hfree Hbnd1 Hbnd2.
+  - (*Fmatch*) rewrite H; auto; try solve[solve_invars Hfree Hbnd1 Hbnd2].
+    simpl. rewrite map_length, Nat.eqb_refl, eq_dec_refl. simpl.
+    rewrite all2_forall with(d1:=(Pwild, Ftrue))(d2:=(Pwild, Ftrue)).
+    2: rewrite map_length; auto.
+    intros i Hi.
+    rewrite map_nth_inbound with (d2:=(Pwild, Ftrue)); auto. simpl.
+    set (t := (nth i ps (Pwild, Ftrue))) in *.
+    (*Results we need*)
+    assert (Hint: In t ps). {
+      apply nth_In; auto.
+    }
+    assert (Hbndi: forall x, In x (pat_fv (fst t)) \/ In x (fmla_bnd (snd t)) ->
+    ~ In (fst x) (map snd l)). {
+      intros. apply Hbnd1; rewrite !in_app_iff, in_concat.
+      right. exists (pat_fv (fst t) ++ fmla_bnd (snd t)).
+      split; [rewrite in_map_iff |
+      rewrite in_app_iff]; auto.
+      exists t. split; auto.
+    }
+    assert (Hfvi: forall x, In x (fmla_fv (snd t)) ->
+      ~ In (fst x) (map snd l)). {
+      intros x Hinx.
+      destruct (in_bool_spec vsymbol_eq_dec x (pat_fv (fst t))); auto.
+      apply Hfree. simpl_set. right.
+      exists t. split; auto. simpl_set; auto.
+    }
+    rewrite a_convert_alpha_p; auto; simpl.
+    rewrite Forall_map in H0.
+    rewrite Forall_forall in H0.
+    unfold add_vals.
+    rewrite a_convert_map_p_fv; auto.
+    replace (combine (pat_fv (fst t))
+    (map (replace_var l) (pat_fv (fst t))) ++
+    mk_alpha_list l bnd) with 
+    (mk_alpha_list l (pat_fv (fst t) ++ bnd)) .
+    2: {
+      unfold mk_alpha_list. rewrite map_app.
+      f_equal.
+      rewrite <- (combine_eq (map _ _)).
+      rewrite !map_map. simpl. f_equal.
+      rewrite map_id; auto.
+    }
+    apply H0; auto.
+    intros x. rewrite in_app_iff; intros [Hx | Hx]; auto.
+Qed.
+
+Lemma replace_var_in l x
+ (* (Hn: NoDup (map snd l))*):
+  In (fst x) (map fst l) ->
+  In ((fst x), (fst (replace_var l x))) l.
+Proof.
+  intros. unfold replace_var.
+  destruct (get_assoc_list string_dec l (fst x)) eqn : Hl; simpl.
+  - apply get_assoc_list_some in Hl.
+    auto.
+  - apply get_assoc_list_none in Hl.
+    contradiction.
+Qed. 
+
+Lemma replace_var_notin l x:
+  ~ In (fst x) (map fst l) ->
+  replace_var l x = x.
+Proof.
+  intros. unfold replace_var.
+  destruct (get_assoc_list string_dec l (fst x)) eqn : Ha; auto.
+  apply get_assoc_list_some in Ha.
+  exfalso.
+  apply H. rewrite in_map_iff. exists (fst x, s). auto.
+Qed.
+
+
+(*And now we show how the bound variables have changed*)
+Lemma a_convert_map_bnd (l: list (string * string))
+  (Hn: NoDup (map snd l))
+  (t: term) (f: formula) :
+  (forall bnd x, In x (tm_bnd (a_convert_map_t l bnd t)) ->
+    ((In x (tm_bnd t) /\ ~ In (fst x) (map fst l)) \/
+    (exists y, In y (tm_bnd t) /\In (fst y, fst x) l))) /\
+  (forall bnd x, In x (fmla_bnd (a_convert_map_f l bnd f)) ->
+    ((In x (fmla_bnd f) /\ ~ In (fst x) (map fst l)) \/
+    (exists y, In y (fmla_bnd f) /\In (fst y, fst x) l))) .
+Proof.
+  revert t f; apply term_formula_ind; simpl; auto.
+  - intros ? ? ? ? ? ?. rewrite !in_concat, map_map.
+    intros. destruct_all.
+    rewrite in_map_iff in H0.
+    destruct_all.
+    rewrite Forall_forall in H.
+    apply H in H1; auto.
+    destruct_all.
+    + left. split; auto. exists (tm_bnd x1). split; auto.
+      rewrite in_map_iff. exists x1; auto.
+    + right. exists x0. split; auto. rewrite in_concat.
+      exists (tm_bnd x1). split; auto. rewrite in_map_iff.
+      exists x1; auto.
+  - intros. rewrite !in_app_iff in H1.
+    destruct_all.
+    + destruct (in_bool_spec string_dec (fst v) (map fst l)).
+      * right. exists v. split; auto. apply replace_var_in; auto.
+      * left. rewrite replace_var_notin; auto.
+    + apply H in H1. destruct_all; [left | right; exists x0];
+      rewrite in_app_iff; auto.
+    + apply H0 in H1; destruct_all; [left | right; exists x0];
+      rewrite in_app_iff; auto.
+  - (*Tif*) intros.
+    rewrite !in_app_iff in H2 |- *.
+    destruct_all; [apply H in H2 | apply H0 in H2 | apply H1 in H2]; destruct_all; auto;
+    right; exists x0; rewrite !in_app_iff; auto.
+  - (*Tmatch*) intros.
+    rewrite in_app_iff in H1 |- *.
+    (*First, deal with first term*)
+    destruct H1.
+    {
+      apply H in H1. destruct_all; [left | right]; auto.
+      exists x0. rewrite in_app_iff; auto.
+    }
+    clear H.
+    (*Now handle recursion*)
+    revert H1. rewrite map_map; simpl; rewrite in_concat; intros.
+    destruct_all. rewrite in_map_iff in H.
+    destruct_all.
+    rewrite Forall_map in H0.
+    rewrite Forall_forall in H0.
+    rewrite !in_app_iff in H1.
+    destruct H1.
+    + (*We know how to handle patterns*)
+      rewrite a_convert_map_p_fv in H; auto.
+      (*Ugn, need these results*)
+      rewrite in_map_iff in H. destruct_all.
+      destruct (in_bool_spec string_dec (fst x0) (map fst l)).
+      * right. exists x0. split; [| apply replace_var_in; auto].
+        rewrite in_app_iff. right. rewrite in_concat.
+        exists (pat_fv (fst x1) ++ tm_bnd (snd x1)).
+        split; auto.
+        rewrite in_map_iff. exists x1; auto.
+        rewrite in_app_iff; auto.
+      * left. rewrite replace_var_notin; auto. split; auto.
+        right. rewrite in_concat. 
+        exists (pat_fv (fst x1) ++ tm_bnd (snd x1)).
+        split; auto.
+        rewrite in_map_iff. exists x1; auto. 
+        rewrite in_app_iff; auto.
+      * (*TODO: need this (do we need this? Maybe not
+        for weaker version of lemma, but whatever)
+          but will need both so lots of annoying
+          induction stuff again - either combine into 1 lemma
+          or try to prove weaker version of pat*) admit.
+    + apply H0 in H; auto.
+      destruct_all.
+      * left. split; auto. right.
+        rewrite in_concat. 
+        exists (pat_fv (fst x1) ++ tm_bnd (snd x1)).
+        split; auto.
+        rewrite in_map_iff. exists x1; auto.
+        rewrite in_app_iff; auto.
+      * right. exists x0. split; auto.
+        rewrite in_app_iff; right.
+        rewrite in_concat. 
+        exists (pat_fv (fst x1) ++ tm_bnd (snd x1)).
+        split; auto.
+        rewrite in_map_iff. exists x1; auto.
+        rewrite in_app_iff; auto.
+  - (*Teps*)
+    intros.
+    destruct_all.
+    + destruct (in_bool_spec string_dec (fst v) (map fst l)).
+      * right. exists v. split; auto. apply replace_var_in; auto.
+      * left. rewrite replace_var_notin; auto.
+    + apply H in H0. destruct_all; [left | right; exists x0]; auto.
 
 End Alpha.
